feat: add BEq to `DTreeMap`/`TreeMap`/`TreeSet` and their extensional variants (#11404)
This PR adds BEq instance for `DTreeMap`/`TreeMap`/`TreeSet` and their
extensional variants and proves lemmas relating it to the equivalence of
hashmaps/equality of extensional variants.

Stacked on top of #11266

src/Std/Data/TreeSet/Raw/Basic.lean
@@ -353,6 +353,11 @@ def inter (t₁ t₂ : Raw α cmp) : Raw α cmp :=
 
 instance : Inter (Raw α cmp) := ⟨inter⟩
 
+@[inherit_doc TreeSet.beq] def beq (t₁ t₂ : Raw α cmp) : Bool :=
+  letI : Ord α := ⟨cmp⟩; TreeMap.Raw.beq t₁.inner t₂.inner
+
+instance : BEq (Raw α cmp) := ⟨beq⟩
+
 /--
 Computes the difference of the given tree sets.
 
