src/Std/Data/DTreeMap/Raw/Lemmas.lean
@@ -3056,6 +3056,36 @@ theorem get!_inter_of_not_mem_left [TransCmp cmp] [Inhabited β] (h₁ : m₁.WF
 
 end Const
 
+section BEq
+variable {m₁ m₂ : Raw α β cmp} [∀ k, BEq (β k)] [LawfulEqCmp cmp] [TransCmp cmp]
+
+theorem Equiv.beq [∀ k, ReflBEq (β k)] (h₁ : m₁.WF) (h₂ : m₂.WF) (h : m₁ ~m m₂) : beq m₁ m₂ :=
+  Impl.Equiv.beq h₁ h₂ h.1
+
+theorem equiv_of_beq [∀ k, LawfulBEq (β k)] (h₁ : m₁.WF) (h₂ : m₂.WF) : beq m₁ m₂ = true → m₁ ~m m₂ := fun hyp =>
+  let : Ord α := ⟨cmp⟩; ⟨Impl.equiv_of_beq h₁.1 h₂.1 hyp⟩
+
+theorem Equiv.beq_congr {m₃ m₄ : Raw α β cmp} (h₁ : m₁.WF) (h₂ : m₂.WF) (h₃ : m₃.WF) (h₄ : m₄.WF) :
+    m₁ ~m m₃ → m₂ ~m m₄ → Raw.beq m₁ m₂ = Raw.beq m₃ m₄ :=
+  fun w1 w2 => Impl.Equiv.beq_congr h₁ h₂ h₃ h₄ w1.1 w2.1
+
+end BEq
+
+section
+variable {β : Type v} {m₁ m₂ : Raw α (fun _ => β) cmp}
+
+theorem Const.Equiv.beq [TransCmp cmp] [BEq β] [ReflBEq β] (h₁ : m₁.WF) (h₂ : m₂.WF) : m₁ ~m m₂ → beq m₁ m₂ :=
+  fun h => Impl.Const.Equiv.beq h₁ h₂ h.1
+
+theorem Const.equiv_of_beq [TransCmp cmp] [LawfulEqCmp cmp] [BEq β] [LawfulBEq β] (h₁ : m₁.WF) (h₂ : m₂.WF) : beq m₁ m₂ = true → m₁ ~m m₂ :=
+  fun hyp => let : Ord α := ⟨cmp⟩; ⟨Impl.Const.equiv_of_beq h₁.1 h₂.1 hyp⟩
+
+theorem Const.Equiv.beq_congr [TransCmp cmp] [BEq β] {m₃ m₄ : Raw α (fun _ => β) cmp} (h₁ : m₁.WF) (h₂ : m₂.WF) (h₃ : m₃.WF) (h₄ : m₄.WF) :
+    m₁ ~m m₃ → m₂ ~m m₄ → Raw.Const.beq m₁ m₂ = Raw.Const.beq m₃ m₄ :=
+  fun w1 w2 => Impl.Const.Equiv.beq_congr h₁ h₂ h₃ h₄ w1.1 w2.1
+
+end
+
 section Diff
 
 variable {t₁ t₂ : Raw α β cmp}
@@ -5295,11 +5325,13 @@ theorem forM_eq [TransCmp cmp] [Monad m] [LawfulMonad m] {f : (a : α) × β a �
 
 theorem any_eq [TransCmp cmp] {p : (a : α) → β a → Bool} (h₁ : t₁.WF) (h₂ : t₂.WF) (h : t₁ ~m t₂) :
     t₁.any p = t₂.any p := by
-  simp only [any, h.forIn_eq h₁ h₂]
+  simp only [any, Impl.any, ForIn.forIn, bind_pure_comp, map_pure, h.1.forIn_eq h₁.1 h₂.1,
+    Id.run_bind]
 
 theorem all_eq [TransCmp cmp] {p : (a : α) → β a → Bool} (h₁ : t₁.WF) (h₂ : t₂.WF) (h : t₁ ~m t₂) :
     t₁.all p = t₂.all p := by
-  simp only [all, h.forIn_eq h₁ h₂]
+  simp only [all, Impl.all, ForIn.forIn, bind_pure_comp, map_pure, h.1.forIn_eq h₁.1 h₂.1,
+    Id.run_bind]
 
 theorem minKey?_eq [TransCmp cmp] (h₁ : t₁.WF) (h₂ : t₂.WF) (h : t₁ ~m t₂) :
     t₁.minKey? = t₂.minKey? :=
