src/Std/Data/TreeSet/Raw/Lemmas.lean
@@ -818,6 +818,20 @@ theorem isEmpty_inter_iff [TransCmp cmp] (h₁ : t₁.WF) (h₂ : t₂.WF) :
 
 end Inter
 
+section
+variable {m₁ m₂ : Raw α cmp}
+
+theorem Equiv.beq [TransCmp cmp] (h₁ : m₁.WF) (h₂ : m₂.WF) (h : m₁ ~m m₂) : beq m₁ m₂ :=
+  TreeMap.Raw.Const.Equiv.beq h₁ h₂ h.1
+
+theorem equiv_of_beq [TransCmp cmp] [LawfulEqCmp cmp] (h₁ : m₁.WF) (h₂ : m₂.WF) (h : m₁ == m₂): m₁ ~m m₂ :=
+  ⟨TreeMap.Raw.Const.equiv_of_beq h₁.1 h₂.1 h⟩
+
+theorem Equiv.beq_congr [TransCmp cmp] {m₃ m₄ : Raw α cmp} (h₁ : m₁.WF) (h₂ : m₂.WF) (h₃ : m₃.WF) (h₄ : m₄.WF) (w₁ : m₁ ~m m₃) (w₂ : m₂ ~m m₄) : (m₁ == m₂) = (m₃ == m₄) :=
+  TreeMap.Raw.Const.Equiv.beq_congr h₁.1 h₂.1 h₃.1 h₄.1 w₁.1 w₂.1
+
+end
+
 section Diff
 
 variable {t₁ t₂ : Raw α cmp}
